theories/UsedIn.v
@@ -1,11 +1,17 @@
+From Equations Require Import
+  Equations
+  .
 From LinearCore Require
   BoundIn
+  Context
   Map
   Term
   .
 From LinearCore Require Import
+  DollarSign
   Invert
   .
+
 
 
 Inductive Term : Term.term -> String.string -> Prop :=
@@ -69,4 +75,120 @@ Proof.
     + intro T. invert T; [apply IHt1 in used_in_body as [v IH] | apply IHt2 in used_in_another_case as [v IH]];
       eexists; (apply Map.union_overriding; [intros ? [] ? []; reflexivity |]); [right | left]. 2: { exact IH. }
       apply Map.minus_minus. split. { exact IH. } intro B. apply not_shadowed. apply BoundIn.pattern_iff. exact B.
+Qed.
+
+
+
+Inductive Indirect : Context.context -> Term.term -> String.string -> Prop :=
+  | ITransitive {context id term leftover} (F : Map.Pop context id term leftover)
+      {name} (transitive : Indirect leftover term name) ownership
+      : Indirect context (Term.Var id ownership) name
+  | IVar context name ownership
+      : Indirect context (Term.Var name ownership) name
+  | IApF {context function name} (used_in_function : Indirect context function name) argument
+      : Indirect context (Term.App function argument) name
+  | IApA {context argument name} (used_in_argument : Indirect context argument name) function
+      : Indirect context (Term.App function argument) name
+  | IFoT {context type name} (used_in_type : Indirect context type name) variable body
+      : Indirect context (Term.For variable type body) name
+  | IFoB {name variable} (not_shadowed : name <> variable) {context body} (used_in_body : Indirect context body name) type
+      : Indirect context (Term.For variable type body) name
+  | ICaB {pattern name} (not_shadowed : forall (B : BoundIn.Pattern pattern name), False)
+      {context body_if_match} (used_in_body : Indirect context body_if_match name) other_cases
+      : Indirect context (Term.Cas pattern body_if_match other_cases) name
+  | ICaO {context other_cases name} (used_in_another_case : Indirect context other_cases name) pattern body_if_match
+      : Indirect context (Term.Cas pattern body_if_match other_cases) name
+  .
+Arguments Indirect context term name.
+
+Lemma indirect_superset {lil t x} (U : Indirect lil t x) {big} (S : Map.Subset lil big)
+  : Indirect big t x.
+Proof.
+  generalize dependent big. induction U; intros.
+  - destruct F as [F R]. eapply ITransitive; [| apply IHU].
+    + split. { apply S. exact F. } apply Map.remove_if_present_remove.
+    + intros k v F'. apply R in F' as [N' F']. apply Map.remove_if_present_remove.
+      split. { exact N'. } apply S. exact F'.
+  - apply IVar.
+  - apply IApF. apply IHU. exact S.
+  - apply IApA. apply IHU. exact S.
+  - apply IFoT. apply IHU. exact S.
+  - apply IFoB. { exact not_shadowed. } apply IHU. exact S.
+  - apply ICaB. { exact not_shadowed. } apply IHU. exact S.
+  - apply ICaO. apply IHU. exact S.
+Qed.
+
+(* NOTE: Depending on the chainedness of the context, this could be powerfully inefficient,
+ * since we aren't marking visited notes to skip later. However, this is easier to prove. *)
+Equations indirect (context : Context.context) (t : Term.term) : Map.set by wf (Nat.add (Term.nodes t) $
+    List.fold_right (fun kv => Nat.add $ Term.nodes $ snd kv) 0 $ MapCore.bindings context) lt :=
+  indirect context (Term.Var name _) with Map.found_dec context name => {
+    | Map.NotFound => Map.singleton name tt
+    | @Map.Found looked_up _ => Map.set_add name $ indirect (Map.remove name context) looked_up };
+  indirect _ (Term.App function argument) :=
+      Map.set_union (indirect context function) (indirect context argument);
+  indirect _ (Term.For variable type body) :=
+      Map.set_union (indirect context type) (Map.remove variable (indirect context body));
+  indirect _ (Term.Cas pattern body_if_match other_cases) :=
+      Map.set_union (indirect context other_cases) (Map.minus (indirect context body_if_match) (BoundIn.pattern pattern));
+  indirect _ _ := Map.empty.
+Next Obligation.
+  clear indirect. assert (BS := Map.bindings_remove_split Y). apply MapCore.bindings_spec1 in Y.
+  destruct BS as [bl [br [-> ->]]]; clear context Y. repeat rewrite List.fold_right_app. cbn.
+  induction bl as [| [k v] tail IH]; cbn in *. { apply PeanoNat.Nat.lt_succ_diag_r. }
+  rewrite PeanoNat.Nat.add_assoc. rewrite (PeanoNat.Nat.add_comm $ Term.nodes looked_up). rewrite plus_n_Sm.
+  rewrite <- PeanoNat.Nat.add_assoc. apply PeanoNat.Nat.add_lt_mono_l. exact IH. Qed.
+Next Obligation.
+  rewrite <- PeanoNat.Nat.add_assoc. rewrite plus_n_Sm. apply PeanoNat.Nat.add_lt_mono_l.
+  rewrite <- PeanoNat.Nat.add_succ_l. apply PeanoNat.Nat.lt_add_pos_l. apply PeanoNat.Nat.lt_0_succ. Qed.
+Next Obligation.
+  rewrite (PeanoNat.Nat.add_comm $ Term.nodes function).
+  rewrite <- PeanoNat.Nat.add_assoc. rewrite plus_n_Sm. apply PeanoNat.Nat.add_lt_mono_l.
+  rewrite <- PeanoNat.Nat.add_succ_l. apply PeanoNat.Nat.lt_add_pos_l. apply PeanoNat.Nat.lt_0_succ. Qed.
+Next Obligation.
+  rewrite <- PeanoNat.Nat.add_assoc. rewrite plus_n_Sm. apply PeanoNat.Nat.add_lt_mono_l.
+  rewrite <- PeanoNat.Nat.add_succ_l. apply PeanoNat.Nat.lt_add_pos_l. apply PeanoNat.Nat.lt_0_succ. Qed.
+Next Obligation.
+  rewrite (PeanoNat.Nat.add_comm $ Term.nodes type).
+  rewrite <- PeanoNat.Nat.add_assoc. rewrite plus_n_Sm. apply PeanoNat.Nat.add_lt_mono_l.
+  rewrite <- PeanoNat.Nat.add_succ_l. apply PeanoNat.Nat.lt_add_pos_l. apply PeanoNat.Nat.lt_0_succ. Qed.
+Next Obligation.
+  rewrite (PeanoNat.Nat.add_comm $ Term.nodes body_if_match).
+  rewrite <- PeanoNat.Nat.add_assoc. rewrite plus_n_Sm. apply PeanoNat.Nat.add_lt_mono_l.
+  rewrite <- PeanoNat.Nat.add_succ_l. apply PeanoNat.Nat.lt_add_pos_l. apply PeanoNat.Nat.lt_0_succ. Qed.
+Next Obligation.
+  rewrite <- PeanoNat.Nat.add_assoc. rewrite plus_n_Sm. apply PeanoNat.Nat.add_lt_mono_l.
+  rewrite <- PeanoNat.Nat.add_succ_l. apply PeanoNat.Nat.lt_add_pos_l. apply PeanoNat.Nat.lt_0_succ. Qed.
+Fail Next Obligation.
+
+Lemma indirect_spec context t
+  : Map.Reflect (Indirect context t) (indirect context t).
+Proof.
+  funelim (indirect context t).
+  - split; intro I. { apply Map.empty_empty in I as []. } invert I.
+  - split; intro I.
+    + apply Map.in_overriding_union in I as [I | I]; [apply H in I | apply H0 in I]; [apply IApF | apply IApA]; exact I.
+    + apply Map.in_overriding_union. invert I; [left | right]; [apply H | apply H0]; assumption.
+  - split; intro I.
+    + apply Map.in_overriding_union in I as [I | I]. { apply H in I. apply IFoT. exact I. }
+      eapply Map.in_remove_if_present in I as [N I]. 2: { apply Map.remove_if_present_remove. }
+      apply IFoB. { exact N. } apply H0. exact I.
+    + apply Map.in_overriding_union. invert I; [left | right]. { apply H. exact used_in_type. }
+      eapply Map.in_remove_if_present. { apply Map.remove_if_present_remove. }
+      split. { exact not_shadowed. } apply H0. exact used_in_body.
+  - split; intro I.
+    + apply Map.in_overriding_union in I as [I | I]. { apply H in I. apply ICaO. exact I. }
+      destruct I as [[] F]. apply Map.minus_minus in F as [F N]. apply ICaB. 2: { apply H0. eexists. exact F. }
+      intro B. apply N. apply BoundIn.pattern_iff. exact B.
+    + apply Map.in_overriding_union. invert I; [right | left]. 2: { apply H. exact used_in_another_case. }
+      exists tt. apply Map.minus_minus. apply H0 in used_in_body as [[] F]. split. { exact F. }
+      intro B. apply not_shadowed. apply BoundIn.pattern_iff. exact B.
+  - split; intro I.
+    + apply Map.in_overriding_add in I as [-> | I]. { constructor. } econstructor. 2: { apply H. exact I. }
+      split. { exact Y. } apply Map.remove_if_present_remove.
+    + apply Map.in_overriding_add. invert I; [right | left]. 2: { reflexivity. }
+      apply H. destruct F as [F R]. destruct (Map.find_det Y F). eapply indirect_superset. { exact transitive. }
+      intros k v F'. apply R in F' as [N' F']. apply Map.remove_if_present_remove. split. { exact N'. } exact F'.
+  - split; intro I. { apply Map.in_singleton in I as ->. constructor. } apply Map.in_singleton.
+    invert I. 2: { reflexivity. } destruct F as [R F]. apply N in R as [].
 Qed.
